@prefix rdf: <http://www.w3.org/1999/02/22-rdf-syntax-ns#> .
@prefix owl: <http://www.w3.org/2002/07/owl#> .
@prefix rdfs: <http://www.w3.org/2000/01/rdf-schema#> .
@prefix oac: <http://www.openannotation.org/ns/> .

<http://www.openannotation.org/ns/>
    a owl:Ontology ;
    owl:versionInfo "alpha3" .

<http://www.openannotation.org/ns/Annotation>
    a rdfs:Class ;
    rdfs:comment "A document identified by an HTTP URI that describes, at least, the Body and Target resources involved in the annotation." ;
    rdfs:isDefinedBy <http://www.openannotation.org/ns/> ;
    rdfs:label "Annotation" .

<http://www.openannotation.org/ns/Body>
    a rdfs:Class ;
    rdfs:comment "The Body is somehow about the Target resource. It is the information which is annotating the Target." ;
    rdfs:isDefinedBy <http://www.openannotation.org/ns/> ;
    rdfs:label "Body" .

<http://www.openannotation.org/ns/ConstrainedBody>
    a rdfs:Class ;
    rdfs:isDefinedBy <http://www.openannotation.org/ns/> ;
    rdfs:label "ConstrainedBody" ;
    rdfs:subClassOf <http://www.openannotation.org/ns/Body> .

<http://www.openannotation.org/ns/ConstrainedTarget>
    a rdfs:Class ;
    rdfs:comment "The ConstrainedTarget is the target of the annotation. It is constrained from another resource (the full resource, of which the target is a part) and constrained by a third resource, the Constraint." ;
    rdfs:isDefinedBy <http://www.openannotation.org/ns/> ;
    rdfs:label "ConstrainedTarget" ;
    rdfs:subClassOf <http://www.openannotation.org/ns/Target> .

<http://www.openannotation.org/ns/Constraint>
    a rdfs:Class ;
    rdfs:comment "The Constraint is a resource which describes how to constrain another resource in a particular way." ;
    rdfs:isDefinedBy <http://www.openannotation.org/ns/> ;
    rdfs:label "Constraint" .

<http://www.openannotation.org/ns/Reply>
    a rdfs:Class ;
    rdfs:comment "A subClass of Annotation which has another Annotation as its Target" ;
    rdfs:isDefinedBy <http://www.openannotation.org/ns/> ;
    rdfs:label "Reply" ;
    rdfs:subClassOf <http://www.openannotation.org/ns/Annotation> .

<http://www.openannotation.org/ns/SvgConstraint>
    a rdfs:Class ;
    rdfs:isDefinedBy <http://www.openannotation.org/ns/> ;
    rdfs:label "SvgConstraint" ;
    rdfs:subClassOf <http://www.openannotation.org/ns/Constraint> .

<http://www.openannotation.org/ns/Target>
    a rdfs:Class ;
    rdfs:comment "The resource that is being annotated" ;
    rdfs:isDefinedBy <http://www.openannotation.org/ns/> ;
    rdfs:label "Target" .

<http://www.openannotation.org/ns/TimeConstraint>
    a rdfs:Class ;
    rdfs:isDefinedBy <http://www.openannotation.org/ns/> ;
    rdfs:label "TimeConstraint" ;
    rdfs:subClassOf <http://www.openannotation.org/ns/Constraint> .

<http://www.openannotation.org/ns/constrainedBy>
    a rdf:Property ;
    rdfs:comment "The relationship from the ConstrainedTarget or ConstrainedBody to the Constraint resource that describes how the full resource is constrained" ;
    rdfs:isDefinedBy <http://www.openannotation.org/ns/> ;
    rdfs:label "constrainedBy" ;
    rdfs:range <http://www.openannotation.org/ns/Constraint> .

<http://www.openannotation.org/ns/constrains>
    a rdf:Property ;
    rdfs:comment "The relationship from the ConstrainedTarget or ConstrainedBody to the full resource being constrained" ;
    rdfs:isDefinedBy <http://www.openannotation.org/ns/> ;
    rdfs:label "constrains" .

<http://www.openannotation.org/ns/hasBody>
    a rdf:Property ;
    rdfs:comment "The relationship between Annotation and Body" ;
    rdfs:domain <http://www.openannotation.org/ns/Annotation> ;
    rdfs:isDefinedBy <http://www.openannotation.org/ns/> ;
    rdfs:label "hasBody" ;
    rdfs:range <http://www.openannotation.org/ns/Body> .

<http://www.openannotation.org/ns/hasTarget>
    a rdf:Property ;
    rdfs:comment "The relationship between Annotation and Target" ;
    rdfs:domain <http://www.openannotation.org/ns/Annotation> ;
    rdfs:isDefinedBy <http://www.openannotation.org/ns/> ;
    rdfs:label "hasTarget" ;
    rdfs:range <http://www.openannotation.org/ns/Target> .

<http://www.openannotation.org/ns/when>
    a rdf:Property ;
    rdfs:comment "The timestamp at which the resource(s) should be interpreted. If attached to an Annotation, it refers to the Content and Targets. If attached to a ConstrainedResource, it refers to the resource which that resource constrains." ;
    rdfs:isDefinedBy <http://www.openannotation.org/ns/> ;
    rdfs:label "when" ;
    rdfs:range rdfs:Literal .

